proofs/hol_light/x86_64/proofs/dump_bytecode.ml
@@ -36,3 +36,7 @@ print_string "==== bytecode end =====================================\n\n";;
 print_string "=== bytecode start: x86_64/mldsa/keccak_f1600_x4_avx2_asm.o ================\n";;
 print_literal_from_elf "x86_64/mldsa/keccak_f1600_x4_avx2_asm.o";;
 print_string "==== bytecode end =====================================\n\n";;
+
+print_string "=== bytecode start: x86_64/mldsa/poly_caddq_avx2_asm.o ================\n";;
+print_literal_from_elf "x86_64/mldsa/poly_caddq_avx2_asm.o";;
+print_string "==== bytecode end =====================================\n\n";;
