proofs/hol_light/x86_64/proofs/subroutine_signatures.ml
@@ -10,6 +10,21 @@
 (* ========================================================================= *)
 
 let subroutine_signatures = [
+("mldsa_poly_caddq_x86",
+  ([(*args*)
+     ("a", "int32_t[static 256]", (*is const?*)"false");
+   ],
+   "void",
+   [(* input buffers *)
+    ("a", "256"(* num elems *), 4(* elem bytesize *));
+   ],
+   [(* output buffers *)
+    ("a", "256"(* num elems *), 4(* elem bytesize *));
+   ],
+   [(* temporary buffers *)
+   ])
+);
+
 ("mldsa_pointwise_x86",
   ([(*args*)
      ("a", "int32_t[static 256]", (*is const?*)"false");
